Change some Vale definitions to enable more memory transformations

vale/code/arch/Vale.Arch.Heap.fst
@@ -11,4 +11,14 @@ let heap_get hi = hi.mh
 let heap_upd hi mh' =
   mi_heap_upd hi mh'
 
-let heap_of_interop ih = ValeHeap (down_mem ih) (Ghost.hide ih)
+let heap_of_interop ih =
+  ValeHeap (down_mem ih) (down_mem ih) (Ghost.hide ih)
+
+let lemma_heap_of_interop (ih:interop_heap) : Lemma
+  (requires True)
+  (ensures _ih (heap_of_interop ih) == ih)
+  [SMTPat (heap_of_interop ih)]
+  =
+  FStar.Pervasives.reveal_opaque (`%_ih) _ih;
+  down_up_identity ih;
+  ()
