vale/code/arch/Vale.Arch.HeapImpl.fst
@@ -8,15 +8,22 @@ open Vale.Interop.Heap_s
 noeq type vale_heap =
   | ValeHeap:
     mh:machine_heap ->
-    ih:Ghost.erased interop_heap{mh == down_mem (Ghost.reveal ih)} ->
+    mh0:machine_heap{is_machine_heap_update mh0 mh} ->
+    ih0:Ghost.erased interop_heap{mh0 == down_mem (Ghost.reveal ih0)} ->
     vale_heap
 
-let _ih (vh:vale_heap) : GTot interop_heap = Ghost.reveal vh.ih
+[@"opaque_to_smt"]
+let _ih (vh:vale_heap) : GTot (ih:interop_heap{vh.mh == down_mem ih}) =
+  let ih0 = Ghost.reveal vh.ih0 in
+  let mh = vh.mh in
+  up_down_identity ih0 mh;
+  up_mem mh ih0
 
 let mi_heap_upd (vh:vale_heap) (mh':machine_heap) : Pure vale_heap
   (requires is_machine_heap_update vh.mh mh')
   (ensures fun vh' -> vh'.mh == mh')
   =
+  let ValeHeap _ mh0 ih0 = vh in
   up_down_identity (_ih vh) mh';
-  ValeHeap mh' (Ghost.hide (up_mem mh' (_ih vh)))
+  ValeHeap mh' mh0 ih0
 
