vale/code/arch/x64/Vale.X64.Decls.fst
@@ -45,7 +45,7 @@ let va_opr_lemma_Mem s base offset b index t =
   let h = M.get_vale_heap s.vs_heap in
   let t = va_opr_code_Mem base offset t in
   M.lemma_valid_mem64 b index h;
-  let OMem (m, t) = t in
+  let OMem (m, t, _) = t in
   assert (valid_buf_maddr64 (eval_maddr m s) h s.vs_memTaint b index t);
   M.lemma_load_mem64 b index h
 
@@ -55,7 +55,7 @@ let va_opr_lemma_Mem128 s base offset t b index =
   let h = M.get_vale_heap s.vs_heap in
   let t = va_opr_code_Mem128 base offset t in
   M.lemma_valid_mem128 b index h;
-  let OMem (m, t) = t in
+  let OMem (m, t, _) = t in
   assert (valid_buf_maddr128 (eval_maddr m s) h s.vs_memTaint b index t);
   M.lemma_load_mem128 b index h
 
